pulse/lib/steel/pulse/Pulse.Checker.Common.fsti
@@ -106,3 +106,9 @@ val intro_comp_typing (g:env)
 val apply_checker_result_k (#g:env) (#ctxt:vprop) (#post_hint:post_hint_for_env g)
   (r:checker_result_t g ctxt (Some post_hint))
   : T.Tac (st_typing_in_ctxt g ctxt (Some post_hint))
+
+val checker_result_for_st_typing (#g:env) (#ctxt:vprop) (#post_hint:post_hint_opt g)
+  (d:st_typing_in_ctxt g ctxt post_hint)
+  : T.Tac (checker_result_t g ctxt post_hint)
+
+
